src/SDK/CMM/CachingCMM.dfy
@@ -1,0 +1,346 @@
+include "../../StandardLibrary/StandardLibrary.dfy"
+include "../../StandardLibrary/UInt.dfy"
+include "Defs.dfy"
+include "../AlgorithmSuite.dfy"
+include "../Materials.dfy"
+include "../../Crypto/Digests.dfy"
+include "../../Crypto/Signature.dfy"
+include "../../Util/Streams.dfy"
+include "../Serialize.dfy"
+include "../MessageHeader.dfy"
+include "../../Util/Time.dfy"
+
+module CachingCMMDef {
+  import opened StandardLibrary
+  import opened UInt = StandardLibrary.UInt
+  import CMMDefs
+  import AlgorithmSuite
+  import Materials
+  import Digests
+  import Signature
+  import Streams
+  import Serialize
+  import MessageHeader
+  import Time
+
+  // The specification says:
+  //  -- the default bytes limit must not exceed 2^63 - 1
+  //  -- the default message limit is 2^32
+  //  -- nothing about the default time-to-live limit
+  const DEFAULT_TIME_TO_LIVE_LIMIT: nat := 3600  // in seconds
+  const DEFAULT_BYTE_USE_LIMIT: uint64 := 0x7FFF_FFFF_FFFF_FFFF  // 2^63 - 1
+  const DEFAULT_MESSAGE_USE_LIMIT: uint64 := 0x1_0000_0000  // 2^32
+
+  const CACHE_ID_HASH_ALGORITHM := Signature.ECDSAParams.ECDSA_P384  // note, ESDK Java uses "SHA-512"
+
+  /* Notes:
+   *
+   * For GetEncryptionMaterials, the specification talks about
+   *     "If a cache entry is found" and
+   *     "If a cache entry is not found"
+   * and says nothing about expiry. For DecryptMaterials, the corresponding specification says
+   *     "If a cache entry is found" and
+   *     "If a cache entry is not found or the cache entry is expired".
+   * The code below considers expiry in all cases. It also considers the indicated bytes and
+   * message-count limits.
+   *
+   * The specification says a Caching CMM MUST have a partition ID, which avoids collisions
+   * when several Caching CMMs share one CMC. This implementation never shares a CMC, so the
+   * partition ID is omitted.
+   *
+   * The Java implementation bypasses the cache in several reasonable ways that are not mentioned
+   * in the specification:
+   *  - Bypass cache when performing streaming operations, unless the stream size is set before
+   *    writing any data.
+   *  - Bypass cache when "plaintextLen" is not specified.
+   * The implementation below also bypasses the cache when "plaintextLen" is not specified.
+   */
+
+  class CachingCMM extends CMMDefs.CMM {
+    const cmm: CMMDefs.CMM
+    const cmc: CryptographicMaterialsCache
+    const timeToLiveLimit: nat  // in seconds
+    const bytesLimit: uint64
+    const messagesLimit: uint64
+
+    predicate Valid()
+      reads this, Repr
+      ensures Valid() ==> this in Repr
+    {
+      this in Repr &&
+      cmm in Repr && cmm.Repr <= Repr && this !in cmm.Repr && cmm.Valid() &&
+      cmc in Repr && cmc.Repr <= Repr && this !in cmc.Repr && cmc.Valid() &&
+      cmm.Repr !! cmc.Repr
+    }
+
+    constructor (cmm: CMMDefs.CMM)
+      requires cmm.Valid()
+      ensures Valid() && fresh(Repr - old(cmm.Repr))
+      ensures this.cmm == cmm
+    {
+      this.timeToLiveLimit := DEFAULT_TIME_TO_LIVE_LIMIT;
+      this.bytesLimit := DEFAULT_BYTE_USE_LIMIT;
+      this.messagesLimit := DEFAULT_MESSAGE_USE_LIMIT;
+
+      this.cmm := cmm;
+      var cmc := new CryptographicMaterialsCache();
+      assert cmc in cmc.Repr;
+      this.cmc := cmc;
+      Repr := {this} + cmm.Repr + cmc.Repr;
+    }
+
+    method GetEncryptionMaterials(encCtx: Materials.EncryptionContext,
+                                  algSuiteID: Option<AlgorithmSuite.ID>,
+                                  plaintextLen: Option<nat>)
+                                  returns (res: Result<Materials.ValidEncryptionMaterials>)
+      requires Valid()
+      requires ValidAAD(encCtx) && Materials.GetKeysFromEncryptionContext(encCtx) !! Materials.ReservedKeyValues
+      modifies Repr
+      ensures Valid() && fresh(Repr - old(Repr))
+      ensures res.Success? ==> |res.value.dataKeyMaterials.plaintextDataKey| == res.value.dataKeyMaterials.algorithmSuiteID.KDFInputKeyLength()
+      ensures res.Success? ==> |res.value.dataKeyMaterials.encryptedDataKeys| > 0
+      ensures res.Success? ==> ValidAAD(res.value.encryptionContext)
+      ensures res.Success? ==>
+        match res.value.dataKeyMaterials.algorithmSuiteID.SignatureType()
+          case None => true
+          case Some(sigType) =>
+            res.value.signingKey.Some? &&
+            Signature.ECDSA.WfSK(sigType, res.value.signingKey.get)
+    {
+      if plaintextLen.None?
+      || bytesLimit as int <= plaintextLen.get
+      || (algSuiteID.Some? && algSuiteID.get.ContainsIdentityKDF())
+      {
+        // So, get encryption materials from the underlying CMM.
+        res := cmm.GetEncryptionMaterials(encCtx, algSuiteID, plaintextLen);
+        Repr := Repr + cmm.Repr;
+        return;
+      }
+
+      var cacheID :- ComputeCacheID(algSuiteID, encCtx);
+
+      var entry := cmc.LookupEncrypt(cacheID);
+      Repr := Repr + cmc.Repr;
+      if entry != null {
+        entry.IncrementUse(plaintextLen.get, 1);
+        var currentTime := Time.GetCurrent();
+        if entry.expiryTime <= currentTime
+        || bytesLimit as nat <= entry.bytesEncrypted
+        || messagesLimit as nat <= entry.messagesEncrypted
+        {
+          // Note, the specification says to treat these numbers as uint64, but the Java ESDK
+          // treats them as signed int64.
+          cmc.EvictEncrypt(cacheID);
+          Repr := Repr + cmc.Repr;
+        } else {
+          return Success(entry.encMat);
+        }
+      }
+
+      // Get encryption materials from the underlying CMM, but use None for the plaintext
+      // length (since the caching returns encryption materials that are independent of
+      // plaintext length).
+      res := cmm.GetEncryptionMaterials(encCtx, algSuiteID, None);
+      Repr := Repr + cmm.Repr;
+      var encMat :- res;
+      // Add them to the cache.
+      entry := cmc.AddEncrypt(cacheID, encMat, DEFAULT_TIME_TO_LIVE_LIMIT);
+      Repr := Repr + cmc.Repr;
+      entry.IncrementUse(plaintextLen.get, 1);
+      return Success(encMat);
+    }
+    method DecryptMaterials(algSuiteID: AlgorithmSuite.ID,
+                            edks: seq<Materials.EncryptedDataKey>,
+                            encCtx: Materials.EncryptionContext)
+                            returns (res: Result<Materials.ValidDecryptionMaterials>)
+      requires Valid() && ValidAAD(encCtx) && |edks| > 0
+      modifies Repr
+      ensures Valid() && fresh(Repr - old(Repr))
+      ensures res.Success? ==>
+        |res.value.plaintextDataKey| == res.value.algorithmSuiteID.KeyLength()
+      ensures res.Success? && res.value.algorithmSuiteID.SignatureType().Some? ==> res.value.verificationKey.Some?
+    {
+      var cacheID :- ComputeCacheID(Some(algSuiteID), encCtx);
+
+      var entry := cmc.LookupDecrypt(cacheID);
+      Repr := Repr + cmc.Repr;
+      if entry != null {
+        var currentTime := Time.GetCurrent();
+        if entry.expiryTime <= currentTime {
+          cmc.EvictDecrypt(cacheID);
+          Repr := Repr + cmc.Repr;
+        } else {
+          return Success(entry.decMat);
+        }
+      }
+
+      // Get decryption materials from the underlying CMM.
+      res := cmm.DecryptMaterials(algSuiteID, edks, encCtx);
+      Repr := Repr + cmm.Repr;
+      var decMat :- res;
+      // Add them to the cache.
+      entry := cmc.AddDecrypt(cacheID, decMat, DEFAULT_TIME_TO_LIVE_LIMIT);
+      Repr := Repr + cmc.Repr;
+      return Success(decMat);
+    }
+  }
+
+
+  method ComputeCacheID(algSuiteID: Option<AlgorithmSuite.ID>, encCtx: Materials.EncryptionContext) returns (res: Result<seq<uint8>>)
+    requires MessageHeader.ValidAAD(encCtx)
+  {
+    var wr := new Streams.StringWriter();
+
+    // Note, if a partition ID were used, write the partition ID hash to wr here
+
+    match algSuiteID {
+      case None =>
+        var _ :- wr.WriteByte(0);
+      case Some(algID) =>
+        var _ :- wr.WriteByte(1);
+        var _ :- wr.WriteUInt16(algID as uint16);
+    }
+
+    var encCtxWr := new Streams.StringWriter();
+    var _ :- Serialize.SerializeAAD(encCtxWr, encCtx);
+    var encCtxEncoding := Signature.Digest(CACHE_ID_HASH_ALGORITHM, encCtxWr.data);
+    var _ :- wr.WriteSeq(encCtxEncoding);
+
+    var cacheID := Signature.Digest(CACHE_ID_HASH_ALGORITHM, wr.data);
+    return Success(cacheID);
+  }
+
+  predicate GoodEncMat(encMat: Materials.EncryptionMaterials) {
+    |encMat.dataKeyMaterials.encryptedDataKeys| > 0 &&
+    MessageHeader.ValidAAD(encMat.encryptionContext) &&
+    match encMat.dataKeyMaterials.algorithmSuiteID.SignatureType()
+      case None => true
+      case Some(sigType) =>
+        encMat.signingKey.Some? &&
+        Signature.ECDSA.WfSK(sigType, encMat.signingKey.get)
+  }
+
+  predicate GoodDecMat(decMat: Materials.DecryptionMaterials) {
+    |decMat.plaintextDataKey| == decMat.algorithmSuiteID.KeyLength() &&
+    (decMat.algorithmSuiteID.SignatureType().Some? ==> decMat.verificationKey.Some?)
+  }
+
+  class CryptographicMaterialsCache {
+    ghost var Repr: set<object>
+    var EM: map<seq<uint8>, CacheEntryEncrypt>
+    var DM: map<seq<uint8>, CacheEntryDecrypt>
+
+    predicate Valid()
+      reads this, Repr
+      ensures Valid() ==> this in Repr
+    {
+      this in Repr &&
+      (forall id :: id in EM.Keys ==> EM[id] in Repr && GoodEncMat(EM[id].encMat)) &&
+      (forall id :: id in DM.Keys ==> DM[id] in Repr && GoodDecMat(DM[id].decMat))
+    }
+
+    constructor ()
+      ensures Valid() && fresh(Repr)
+    {
+      Repr, EM, DM := {this}, map[], map[];
+    }
+
+    function method LookupEncrypt(cacheID: seq<uint8>): (entry: CacheEntryEncrypt?)
+      requires Valid()
+      reads Repr
+      ensures entry != null ==> entry in Repr && GoodEncMat(entry.encMat)
+    {
+      if cacheID in EM.Keys then EM[cacheID] else null
+    }
+
+    function method LookupDecrypt(cacheID: seq<uint8>): (entry: CacheEntryDecrypt?)
+      requires Valid()
+      reads Repr
+      ensures entry != null ==> entry in Repr && GoodDecMat(entry.decMat)
+    {
+      if cacheID in DM.Keys then DM[cacheID] else null
+    }
+
+    // Adds an entry [cacheID := encMat] to the cache, replacing any previous encrypt entry for cacheID
+    // and initializing usage limits to (currentTime + timeToLiveLimit, 0, 0). Returns the resulting entry.
+    method AddEncrypt(cacheID: seq<uint8>, encMat: Materials.ValidEncryptionMaterials, timeToLiveLimit: nat) returns (entry: CacheEntryEncrypt)
+      requires Valid() && GoodEncMat(encMat) && 0 < timeToLiveLimit
+      modifies Repr
+      ensures Valid() && fresh(Repr - old(Repr)) && entry in Repr
+    {
+      entry := new CacheEntryEncrypt(encMat, timeToLiveLimit);
+      Repr := Repr + {entry};
+      EM := EM[cacheID := entry];
+    }
+
+    // Adds an entry [cacheID := decMat] to the cache, replacing any previous decrypt entry for cacheID
+    // and initializing usage limits to (currentTime + timeToLiveLimit). Returns the resulting entry.
+    method AddDecrypt(cacheID: seq<uint8>, decMat: Materials.ValidDecryptionMaterials, timeToLiveLimit: nat) returns (entry: CacheEntryDecrypt)
+      requires Valid() && GoodDecMat(decMat) && 0 < timeToLiveLimit
+      modifies Repr
+      ensures Valid() && fresh(Repr - old(Repr)) && entry in Repr
+    {
+      entry := new CacheEntryDecrypt(decMat, timeToLiveLimit);
+      Repr := Repr + {entry};
+      DM := DM[cacheID := entry];
+    }
+
+    // Removes any encrypt entry for cacheID.
+    method EvictEncrypt(cacheID: seq<uint8>)
+      requires Valid()
+      modifies Repr
+      ensures Valid() && fresh(Repr - old(Repr))
+    {
+      EM := map id | id in EM.Keys && id != cacheID :: EM[id];
+    }
+
+    // Removes any decrypt entry for cacheID.
+    method EvictDecrypt(cacheID: seq<uint8>)
+      requires Valid()
+      modifies Repr
+      ensures Valid() && fresh(Repr - old(Repr))
+    {
+      DM := map id | id in DM.Keys && id != cacheID :: DM[id];
+    }
+  }
+
+  class CacheEntryEncrypt {
+    const encMat: Materials.ValidEncryptionMaterials
+    const expiryTime: nat
+    var messagesEncrypted: nat
+    var bytesEncrypted: nat
+
+    constructor (encMat: Materials.ValidEncryptionMaterials, timeToLiveLimit: nat)
+      ensures messagesEncrypted == bytesEncrypted == 0
+      ensures this.encMat == encMat
+    {
+      this.encMat := encMat;
+      var currentTime := Time.GetCurrent();
+      expiryTime := currentTime + timeToLiveLimit;
+      messagesEncrypted, bytesEncrypted := 0, 0;
+    }
+
+    method IncrementUse(byteCount: nat, useCount: nat)
+      modifies this
+      ensures messagesEncrypted == old(messagesEncrypted) + byteCount
+      ensures bytesEncrypted == old(bytesEncrypted) + useCount
+    {
+      messagesEncrypted := messagesEncrypted + byteCount;
+      bytesEncrypted := bytesEncrypted + useCount;
+    }
+  }
+
+
+  class CacheEntryDecrypt {
+    const decMat: Materials.ValidDecryptionMaterials
+    const expiryTime: nat
+
+    constructor (decMat: Materials.ValidDecryptionMaterials, timeToLiveLimit: nat)
+      ensures this.decMat == decMat
+    {
+      this.decMat := decMat;
+      var currentTime := Time.GetCurrent();
+      expiryTime := currentTime + timeToLiveLimit;
+    }
+  }
+}
