src/SDK/CMM/DefaultCMM.dfy
@@ -26,6 +26,7 @@ module DefaultCMMDef {
 
     predicate Valid()
       reads this, Repr
+      ensures Valid() ==> this in Repr
     {
       kr in Repr &&
       Repr == {this, kr} + kr.Repr &&
