src/Util/Time.dfy
@@ -1,0 +1,4 @@
+module Time {
+  // Returns the number of seconds since the Unix epoch
+  method {:extern "TimeUtil.Time", "CurrentTime"} GetCurrent() returns (seconds: nat)
+}
